<?xml version="1.0"?>
<rdf:RDF xmlns="http://www.semanticweb.org/nazanin/ontologies/2025/Fairtology_L1#"
     xml:base="http://www.semanticweb.org/nazanin/ontologies/2025/Fairtology_L1"
     xmlns:owl="http://www.w3.org/2002/07/owl#"
     xmlns:rdf="http://www.w3.org/1999/02/22-rdf-syntax-ns#"
     xmlns:xml="http://www.w3.org/XML/1998/namespace"
     xmlns:xsd="http://www.w3.org/2001/XMLSchema#"
     xmlns:rdfs="http://www.w3.org/2000/01/rdf-schema#">
    <owl:Ontology rdf:about="http://www.semanticweb.org/nazanin/ontologies/2025/Fairtology_L1">
        <rdfs:comment>An ontology for modeling structural and thematic elements of global fairy tales, including character archetypes, moral themes, and narrative outcomes.</rdfs:comment>
    </owl:Ontology>
    


    <!-- 
    ///////////////////////////////////////////////////////////////////////////////////////
    //
    // Object Properties
    //
    ///////////////////////////////////////////////////////////////////////////////////////
     -->

    


    <!-- http://www.semanticweb.org/nazanin/ontologies/2025/Fairtology_L1#ReceivedBy -->

    <owl:ObjectProperty rdf:about="http://www.semanticweb.org/nazanin/ontologies/2025/Fairtology_L1#ReceivedBy">
        <rdfs:domain rdf:resource="http://www.semanticweb.org/nazanin/ontologies/2025/Fairtology_L1#Fairytale"/>
        <rdfs:range rdf:resource="http://www.semanticweb.org/nazanin/ontologies/2025/Fairtology_L1#Audience"/>
        <rdfs:comment>Connects to target audience type or group.</rdfs:comment>
    </owl:ObjectProperty>
    


    <!-- http://www.semanticweb.org/nazanin/ontologies/2025/Fairtology_L1#hasCharacterType -->

    <owl:ObjectProperty rdf:about="http://www.semanticweb.org/nazanin/ontologies/2025/Fairtology_L1#hasCharacterType">
        <rdfs:domain rdf:resource="http://www.semanticweb.org/nazanin/ontologies/2025/Fairtology_L1#Fairytale"/>
        <rdfs:range rdf:resource="http://www.semanticweb.org/nazanin/ontologies/2025/Fairtology_L#CharacterArchetype"/>
        <rdfs:comment>Links a tale to a character archetype involved.</rdfs:comment>
    </owl:ObjectProperty>
    


    <!-- http://www.semanticweb.org/nazanin/ontologies/2025/Fairtology_L1#hasEndingType -->

    <owl:ObjectProperty rdf:about="http://www.semanticweb.org/nazanin/ontologies/2025/Fairtology_L1#hasEndingType">
        <rdfs:domain rdf:resource="http://www.semanticweb.org/nazanin/ontologies/2025/Fairtology_L1#Plot"/>
        <rdfs:range rdf:resource="http://www.semanticweb.org/nazanin/ontologies/2025/Fairtology_L1#EndingType"/>
        <rdfs:comment>Links a tale to its ending resolution type.</rdfs:comment>
    </owl:ObjectProperty>
    


    <!-- http://www.semanticweb.org/nazanin/ontologies/2025/Fairtology_L1#hasLiteraryMode -->

    <owl:ObjectProperty rdf:about="http://www.semanticweb.org/nazanin/ontologies/2025/Fairtology_L1#hasLiteraryMode">
        <rdfs:domain rdf:resource="http://www.semanticweb.org/nazanin/ontologies/2025/Fairtology_L1#Fairytale"/>
        <rdfs:range rdf:resource="http://www.semanticweb.org/nazanin/ontologies/2025/Fairtology_L1#LiteraryMode"/>
    </owl:ObjectProperty>
    


    <!-- http://www.semanticweb.org/nazanin/ontologies/2025/Fairtology_L1#hasMoralTheme -->

    <owl:ObjectProperty rdf:about="http://www.semanticweb.org/nazanin/ontologies/2025/Fairtology_L1#hasMoralTheme">
        <rdfs:domain rdf:resource="http://www.semanticweb.org/nazanin/ontologies/2025/Fairtology_L1#Fairytale"/>
        <rdfs:range rdf:resource="http://www.semanticweb.org/nazanin/ontologies/2025/Fairtology_L1#MoralTheme"/>
        <rdfs:comment>Links a tale to the moral lesson it conveys.</rdfs:comment>
    </owl:ObjectProperty>
    


    <!-- http://www.semanticweb.org/nazanin/ontologies/2025/Fairtology_L1#hasNarrativeStructure -->

    <owl:ObjectProperty rdf:about="http://www.semanticweb.org/nazanin/ontologies/2025/Fairtology_L1#hasNarrativeStructure">
        <rdfs:domain rdf:resource="http://www.semanticweb.org/nazanin/ontologies/2025/Fairtology_L1#Plot"/>
        <rdfs:range rdf:resource="http://www.semanticweb.org/nazanin/ontologies/2025/Fairtology_L1#RecurringNarrativeStructure"/>
    </owl:ObjectProperty>
    


    <!-- 
    ///////////////////////////////////////////////////////////////////////////////////////
    //
    // Data properties
    //
    ///////////////////////////////////////////////////////////////////////////////////////
     -->

    


    <!-- http://www.semanticweb.org/nazanin/ontologies/2025/Fairtology_L1#hasValue -->

    <owl:DatatypeProperty rdf:about="http://www.semanticweb.org/nazanin/ontologies/2025/Fairtology_L1#hasValue">
        <rdf:type rdf:resource="http://www.w3.org/2002/07/owl#FunctionalProperty"/>
        <rdfs:domain>
            <owl:Class>
                <owl:unionOf rdf:parseType="Collection">
                    <rdf:Description rdf:about="http://www.semanticweb.org/nazanin/ontologies/2025/Fairtology_L1#MoralTheme"/>
                    <rdf:Description rdf:about="http://www.semanticweb.org/nazanin/ontologies/2025/Fairtology_L1#Plot"/>
                    <rdf:Description rdf:about="https://ontology.golemlab.eu/G1_Character"/>
                </owl:unionOf>
            </owl:Class>
        </rdfs:domain>
        <rdfs:range rdf:resource="http://www.w3.org/2001/XMLSchema#string"/>
        <rdfs:comment>Plot of the Fairy tale or Moral theme contain strings</rdfs:comment>
        <rdfs:label xml:lang="en">hasValue</rdfs:label>
    </owl:DatatypeProperty>
    


    <!-- 
    ///////////////////////////////////////////////////////////////////////////////////////
    //
    // Classes
    //
    ///////////////////////////////////////////////////////////////////////////////////////
     -->

    


    <!-- http://www.semanticweb.org/nazanin/ontologies/2025/Fairtology_L#CharacterArchetype -->

    <owl:Class rdf:about="http://www.semanticweb.org/nazanin/ontologies/2025/Fairtology_L#CharacterArchetype">
        <rdfs:comment>Represents common character roles in fairy tales which were modeled based on a  simplified set of narrative character roles commonly found in fairy tales. This model draws conceptually from Northrop Frye&apos;s theory of literary archetypes but adapts it to the domain of folk and fairy tale ontology.</rdfs:comment>
    </owl:Class>
    


    <!-- http://www.semanticweb.org/nazanin/ontologies/2025/Fairtology_L1#Audience -->

    <owl:Class rdf:about="http://www.semanticweb.org/nazanin/ontologies/2025/Fairtology_L1#Audience">
        <rdfs:comment>Refers to the intended or actual viewers/readers of the tale.</rdfs:comment>
    </owl:Class>
    


    <!-- http://www.semanticweb.org/nazanin/ontologies/2025/Fairtology_L1#BittersweetEnding -->

    <owl:Class rdf:about="http://www.semanticweb.org/nazanin/ontologies/2025/Fairtology_L1#BittersweetEnding">
        <rdfs:subClassOf rdf:resource="http://www.semanticweb.org/nazanin/ontologies/2025/Fairtology_L1#EndingType"/>
        <rdfs:comment>Mixed resolution involving growth through loss or sacrifice.</rdfs:comment>
    </owl:Class>
    


    <!-- http://www.semanticweb.org/nazanin/ontologies/2025/Fairtology_L1#Departure -->

    <owl:Class rdf:about="http://www.semanticweb.org/nazanin/ontologies/2025/Fairtology_L1#Departure">
        <rdfs:subClassOf rdf:resource="http://www.semanticweb.org/nazanin/ontologies/2025/Fairtology_L1#RecurringNarrativeStructure"/>
        <rdfs:comment>The hero leaves home or normality, usually to face a challenge or enter a magical realm. Corresponds to Propp’s function of &apos;absentation&apos;.</rdfs:comment>
    </owl:Class>
    


    <!-- http://www.semanticweb.org/nazanin/ontologies/2025/Fairtology_L1#EndingType -->

    <owl:Class rdf:about="http://www.semanticweb.org/nazanin/ontologies/2025/Fairtology_L1#EndingType">
        <rdfs:comment>Denotes the resolution structure or emotional closure of the story.</rdfs:comment>
    </owl:Class>
    


    <!-- http://www.semanticweb.org/nazanin/ontologies/2025/Fairtology_L1#Fairytale -->

    <owl:Class rdf:about="http://www.semanticweb.org/nazanin/ontologies/2025/Fairtology_L1#Fairytale">
        <rdfs:comment>Represents the original fairy tale narratives.</rdfs:comment>
    </owl:Class>
    


    <!-- http://www.semanticweb.org/nazanin/ontologies/2025/Fairtology_L1#HappilyEverAfter -->

    <owl:Class rdf:about="http://www.semanticweb.org/nazanin/ontologies/2025/Fairtology_L1#HappilyEverAfter">
        <rdfs:subClassOf rdf:resource="http://www.semanticweb.org/nazanin/ontologies/2025/Fairtology_L1#EndingType"/>
        <rdfs:comment>Positive resolution, often involving marriage or restoration.</rdfs:comment>
    </owl:Class>
    


    <!-- http://www.semanticweb.org/nazanin/ontologies/2025/Fairtology_L1#Helper -->

    <owl:Class rdf:about="http://www.semanticweb.org/nazanin/ontologies/2025/Fairtology_L1#Helper">
        <rdfs:subClassOf rdf:resource="http://www.semanticweb.org/nazanin/ontologies/2025/Fairtology_L#CharacterArchetype"/>
        <rdfs:comment>Supports the hero through guidance or gifts.</rdfs:comment>
    </owl:Class>
    


    <!-- http://www.semanticweb.org/nazanin/ontologies/2025/Fairtology_L1#Hero -->

    <owl:Class rdf:about="http://www.semanticweb.org/nazanin/ontologies/2025/Fairtology_L1#Hero">
        <rdfs:subClassOf rdf:resource="http://www.semanticweb.org/nazanin/ontologies/2025/Fairtology_L#CharacterArchetype"/>
        <rdfs:comment>Central figure on a quest or journey.</rdfs:comment>
    </owl:Class>
    


    <!-- http://www.semanticweb.org/nazanin/ontologies/2025/Fairtology_L1#IronicMode -->

    <owl:Class rdf:about="http://www.semanticweb.org/nazanin/ontologies/2025/Fairtology_L1#IronicMode">
        <rdfs:subClassOf rdf:resource="http://www.semanticweb.org/nazanin/ontologies/2025/Fairtology_L1#LiteraryMode"/>
        <rdfs:comment>A narrative where the characters are below the audience in knowledge or power; emphasizes irony, futility, or ambiguity.</rdfs:comment>
    </owl:Class>
    


    <!-- http://www.semanticweb.org/nazanin/ontologies/2025/Fairtology_L1#LiteraryMode -->

    <owl:Class rdf:about="http://www.semanticweb.org/nazanin/ontologies/2025/Fairtology_L1#LiteraryMode">
        <rdfs:comment>Narrative mode expressing the symbolic or emotional tone of a tale. Adapted from Frye’s typology of literary modes.</rdfs:comment>
    </owl:Class>
    


    <!-- http://www.semanticweb.org/nazanin/ontologies/2025/Fairtology_L1#MagicalAid -->

    <owl:Class rdf:about="http://www.semanticweb.org/nazanin/ontologies/2025/Fairtology_L1#MagicalAid">
        <rdfs:subClassOf rdf:resource="http://www.semanticweb.org/nazanin/ontologies/2025/Fairtology_L1#RecurringNarrativeStructure"/>
        <rdfs:comment>A supernatural helper, object, or force assists the hero. Reflects Propp’s &apos;donor&apos; and &apos;magical agent&apos; functions.</rdfs:comment>
    </owl:Class>
    


    <!-- http://www.semanticweb.org/nazanin/ontologies/2025/Fairtology_L1#MoralTheme -->

    <owl:Class rdf:about="http://www.semanticweb.org/nazanin/ontologies/2025/Fairtology_L1#MoralTheme">
        <rdfs:comment>Captures the ethical teachings conveyed through the narratives.</rdfs:comment>
    </owl:Class>
    


    <!-- http://www.semanticweb.org/nazanin/ontologies/2025/Fairtology_L1#MythicMode -->

    <owl:Class rdf:about="http://www.semanticweb.org/nazanin/ontologies/2025/Fairtology_L1#MythicMode">
        <rdfs:subClassOf rdf:resource="http://www.semanticweb.org/nazanin/ontologies/2025/Fairtology_L1#LiteraryMode"/>
        <rdfs:comment>A narrative mode where characters are gods or superhuman beings; the setting is cosmic and timeless.</rdfs:comment>
    </owl:Class>
    


    <!-- http://www.semanticweb.org/nazanin/ontologies/2025/Fairtology_L1#NarrativeUnit -->

    <owl:Class rdf:about="http://www.semanticweb.org/nazanin/ontologies/2025/Fairtology_L1#NarrativeUnit">
        <owl:equivalentClass rdf:resource="https://ontology.golemlab.eu/G7_Narrative_Sequence"/>
        <rdfs:comment>refers to various types of organisation of narrative units and events, including causal and temporal structures, which is essential for understanding narrative coherence.</rdfs:comment>
        <rdfs:label>NarrativeUnit</rdfs:label>
    </owl:Class>
    


    <!-- http://www.semanticweb.org/nazanin/ontologies/2025/Fairtology_L1#Plot -->

    <owl:Class rdf:about="http://www.semanticweb.org/nazanin/ontologies/2025/Fairtology_L1#Plot">
        <rdfs:subClassOf rdf:resource="http://www.semanticweb.org/nazanin/ontologies/2025/Fairtology_L1#Fairytale"/>
        <rdfs:comment>Encapsulates the overall designed arrangement of story elements to produce an emotional or thematic effect.</rdfs:comment>
    </owl:Class>
    


    <!-- http://www.semanticweb.org/nazanin/ontologies/2025/Fairtology_L1#RecurringNarrativeStructure -->

    <owl:Class rdf:about="http://www.semanticweb.org/nazanin/ontologies/2025/Fairtology_L1#RecurringNarrativeStructure">
        <rdfs:subClassOf rdf:resource="http://www.semanticweb.org/nazanin/ontologies/2025/Fairtology_L1#NarrativeUnit"/>
        <rdfs:comment>A commonly repeated narrative configuration or structural pattern found across multiple fairy tales (e.g., departure, magical aid, transformation). Aligned with Vladimir Propp’s 31 narrative functions</rdfs:comment>
        <rdfs:label>RecurringNarrativeStructure</rdfs:label>
    </owl:Class>
    


    <!-- http://www.semanticweb.org/nazanin/ontologies/2025/Fairtology_L1#ReturnAndReward -->

    <owl:Class rdf:about="http://www.semanticweb.org/nazanin/ontologies/2025/Fairtology_L1#ReturnAndReward">
        <rdfs:subClassOf rdf:resource="http://www.semanticweb.org/nazanin/ontologies/2025/Fairtology_L1#RecurringNarrativeStructure"/>
        <rdfs:comment>The hero returns and is recognized or rewarded. Reflects Propp’s &apos;recognition&apos;, &apos;wedding&apos;, or &apos;punishment&apos; stages.</rdfs:comment>
    </owl:Class>
    


    <!-- http://www.semanticweb.org/nazanin/ontologies/2025/Fairtology_L1#RomanticMode -->

    <owl:Class rdf:about="http://www.semanticweb.org/nazanin/ontologies/2025/Fairtology_L1#RomanticMode">
        <rdfs:subClassOf rdf:resource="http://www.semanticweb.org/nazanin/ontologies/2025/Fairtology_L1#LiteraryMode"/>
        <rdfs:comment>A narrative mode in which the hero operates above ordinary limitations; idealized, heroic, or magical.</rdfs:comment>
    </owl:Class>
    


    <!-- http://www.semanticweb.org/nazanin/ontologies/2025/Fairtology_L1#TestOrTrial -->

    <owl:Class rdf:about="http://www.semanticweb.org/nazanin/ontologies/2025/Fairtology_L1#TestOrTrial">
        <rdfs:subClassOf rdf:resource="http://www.semanticweb.org/nazanin/ontologies/2025/Fairtology_L1#RecurringNarrativeStructure"/>
        <rdfs:comment>The protagonist faces challenges or obstacles to prove worth or readiness. Corresponds to Propp’s &apos;interdiction&apos;, &apos;violation&apos;, and &apos;struggle&apos;.</rdfs:comment>
    </owl:Class>
    


    <!-- http://www.semanticweb.org/nazanin/ontologies/2025/Fairtology_L1#TragicEnding -->

    <owl:Class rdf:about="http://www.semanticweb.org/nazanin/ontologies/2025/Fairtology_L1#TragicEnding">
        <rdfs:subClassOf rdf:resource="http://www.semanticweb.org/nazanin/ontologies/2025/Fairtology_L1#EndingType"/>
        <rdfs:comment>Negative outcome involving loss or death.</rdfs:comment>
    </owl:Class>
    


    <!-- http://www.semanticweb.org/nazanin/ontologies/2025/Fairtology_L1#TragicMode -->

    <owl:Class rdf:about="http://www.semanticweb.org/nazanin/ontologies/2025/Fairtology_L1#TragicMode">
        <rdfs:subClassOf rdf:resource="http://www.semanticweb.org/nazanin/ontologies/2025/Fairtology_L1#LiteraryMode"/>
        <rdfs:comment>A narrative where the protagonist falls from a high position due to fate or personal flaw; evokes pity and fear.</rdfs:comment>
    </owl:Class>
    


    <!-- http://www.semanticweb.org/nazanin/ontologies/2025/Fairtology_L1#Transformation -->

    <owl:Class rdf:about="http://www.semanticweb.org/nazanin/ontologies/2025/Fairtology_L1#Transformation">
        <rdfs:subClassOf rdf:resource="http://www.semanticweb.org/nazanin/ontologies/2025/Fairtology_L1#RecurringNarrativeStructure"/>
        <rdfs:comment>A change of form, status, or understanding occurs. Reflects Propp’s &apos;transfiguration&apos;.</rdfs:comment>
    </owl:Class>
    


    <!-- http://www.semanticweb.org/nazanin/ontologies/2025/Fairtology_L1#Trickster -->

    <owl:Class rdf:about="http://www.semanticweb.org/nazanin/ontologies/2025/Fairtology_L1#Trickster">
        <rdfs:subClassOf rdf:resource="http://www.semanticweb.org/nazanin/ontologies/2025/Fairtology_L#CharacterArchetype"/>
        <rdfs:comment>Character who disrupts or subverts norms through cleverness.</rdfs:comment>
    </owl:Class>
    


    <!-- http://www.semanticweb.org/nazanin/ontologies/2025/Fairtology_L1#Villain -->

    <owl:Class rdf:about="http://www.semanticweb.org/nazanin/ontologies/2025/Fairtology_L1#Villain">
        <rdfs:subClassOf rdf:resource="http://www.semanticweb.org/nazanin/ontologies/2025/Fairtology_L#CharacterArchetype"/>
        <rdfs:comment>Antagonist who creates conflict or danger.</rdfs:comment>
    </owl:Class>
    


    <!-- https://ontology.golemlab.eu/G1_Character -->

    <owl:Class rdf:about="https://ontology.golemlab.eu/G1_Character">
        <rdfs:subClassOf rdf:resource="http://www.semanticweb.org/nazanin/ontologies/2025/Fairtology_L1#Fairytale"/>
        <rdfs:comment>“Character is a text- or media-based figure in a storyworld, usually human or human-like,” understood through readers’ knowledge of real people (Jannidis, 2019). Readers attribute to characters mental states such as intentions and beliefs, and consider them to engage in actions. Characters can have specific functional roles within narratives, such as protagonist or antagonist, influencing how readers perceive and interpret the story.</rdfs:comment>
        <rdfs:label>Character</rdfs:label>
    </owl:Class>
    


    <!-- https://ontology.golemlab.eu/G7_Narrative_Sequence -->

    <owl:Class rdf:about="https://ontology.golemlab.eu/G7_Narrative_Sequence">
        <rdfs:comment>G7_Narrative_Sequences can take various forms, including sequences of functions, such as Proppian functions (Propp, 1968), sequences of motifs, or hyleme sequences like fabula and syuzhet. Specifically, a type of narrative sequence is fabula, which refers to the sequence of events of a narrative in chronological and causal order (Abbott, 2019). It represents the underlying structure of the story or what happens in it. Since the concept of fabula is mainly defined in relation to that of syuzhet, its conceptual function is to express a specific ordering of some narrative units. Accordingly, the fabula is a sequence (rdf:Seq) of narrative units (gc:G9) that orders (dlp:sequences) a set of temporal entities called events (dlp: perdurant). Another type is syuzhet, often translated as &quot;plot&quot; or “discourse”. Syuzhet encompasses how events are presented and organized within a narrative (Kukkonen, 2019; Abbott, 2019). It involves the specific ordering and techniques used to articulate the story, reflecting the author’s design and organization to achieve particular aesthetic and cognitive-emotional effects, like suspense. As for fabula, the conceptual function of syuzhet is to express a specific ordering of some narrative units. Accordingly, the syuzhet is a sequence (rdf:Seq) of narrative units (gc:G9) that orders (dlp:sequences) a set of temporal entities called events (dlp: perdurant).</rdfs:comment>
        <rdfs:isDefinedBy>GOLEM Ontology: Graphs and Ontologies for Literary Evolution Models</rdfs:isDefinedBy>
    </owl:Class>
    


    <!-- 
    ///////////////////////////////////////////////////////////////////////////////////////
    //
    // Individuals
    //
    ///////////////////////////////////////////////////////////////////////////////////////
     -->

    


    <!-- http://example.org/fairtale#Departure_SnowWhite -->

    <owl:NamedIndividual rdf:about="http://example.org/fairtale#Departure_SnowWhite">
        <rdf:type rdf:resource="http://www.semanticweb.org/nazanin/ontologies/2025/Fairtology_L1#Departure"/>
        <rdfs:label>Snow White flees into the forest to escape the Queen.</rdfs:label>
    </owl:NamedIndividual>
    


    <!-- http://example.org/fairtale#MagicalAid_Jack -->

    <owl:NamedIndividual rdf:about="http://example.org/fairtale#MagicalAid_Jack">
        <rdf:type rdf:resource="http://www.semanticweb.org/nazanin/ontologies/2025/Fairtology_L1#MagicalAid"/>
        <rdfs:label>Jack receives magical beans that lead to adventure and transformation.</rdfs:label>
    </owl:NamedIndividual>
    


    <!-- http://example.org/fairtale#ReturnAndReward_Rapunzel -->

    <owl:NamedIndividual rdf:about="http://example.org/fairtale#ReturnAndReward_Rapunzel">
        <rdf:type rdf:resource="http://www.semanticweb.org/nazanin/ontologies/2025/Fairtology_L1#ReturnAndReward"/>
        <rdfs:label>Rapunzel is reunited with her prince and gains a peaceful life.</rdfs:label>
    </owl:NamedIndividual>
    


    <!-- http://example.org/fairtale#TestOrTrial_Cinderella -->

    <owl:NamedIndividual rdf:about="http://example.org/fairtale#TestOrTrial_Cinderella">
        <rdf:type rdf:resource="http://www.semanticweb.org/nazanin/ontologies/2025/Fairtology_L1#TestOrTrial"/>
        <rdfs:label>Cinderella must prove her identity and worth through attending the ball.</rdfs:label>
    </owl:NamedIndividual>
    


    <!-- http://example.org/fairtale#Transformation_Beast -->

    <owl:NamedIndividual rdf:about="http://example.org/fairtale#Transformation_Beast">
        <rdf:type rdf:resource="http://www.semanticweb.org/nazanin/ontologies/2025/Fairtology_L1#Transformation"/>
        <rdfs:label>The Beast becomes a prince after Belle&apos;s love breaks the spell.</rdfs:label>
    </owl:NamedIndividual>
</rdf:RDF>



<!-- Generated by the OWL API (version 4.5.29.2024-05-13T12:11:03Z) https://github.com/owlcs/owlapi -->

