<?xml version="1.0"?>
<rdf:RDF xmlns="http://www.semanticweb.org/nazanin/ontologies/2025/Fairtology_L1#"
     xml:base="http://www.semanticweb.org/nazanin/ontologies/2025/Fairtology_L1"
     xmlns:owl="http://www.w3.org/2002/07/owl#"
     xmlns:rdf="http://www.w3.org/1999/02/22-rdf-syntax-ns#"
     xmlns:xml="http://www.w3.org/XML/1998/namespace"
     xmlns:xsd="http://www.w3.org/2001/XMLSchema#"
     xmlns:rdfs="http://www.w3.org/2000/01/rdf-schema#">
    <owl:Ontology rdf:about="http://www.semanticweb.org/nazanin/ontologies/2025/Fairtology_L1">
        <rdfs:comment>An ontology for modeling structural and thematic elements of global fairy tales, including character archetypes, moral themes, and narrative outcomes.</rdfs:comment>
    </owl:Ontology>
    


    <!-- 
    ///////////////////////////////////////////////////////////////////////////////////////
    //
    // Object Properties
    //
    ///////////////////////////////////////////////////////////////////////////////////////
     -->

    


    <!-- http://www.semanticweb.org/nazanin/ontologies/2025/Fairtology_L1#hasCharacterArchetype -->

    <owl:ObjectProperty rdf:about="http://www.semanticweb.org/nazanin/ontologies/2025/Fairtology_L1#hasCharacterArchetype">
        <rdfs:domain rdf:resource="http://example.org/fairytale#Fairytale"/>
        <rdfs:range rdf:resource="http://example.org/fairytale#CharacterArchetype"/>
        <rdfs:comment>Links a tale to a character archetype involved.</rdfs:comment>
    </owl:ObjectProperty>
    


    <!-- http://www.semanticweb.org/nazanin/ontologies/2025/Fairtology_L1#hasEndingType -->

    <owl:ObjectProperty rdf:about="http://www.semanticweb.org/nazanin/ontologies/2025/Fairtology_L1#hasEndingType">
        <rdfs:domain rdf:resource="http://example.org/fairytale#Fairytale"/>
        <rdfs:range rdf:resource="http://example.org/fairytale#EndingType"/>
        <rdfs:comment>Links a tale to its ending resolution type.</rdfs:comment>
    </owl:ObjectProperty>
    


    <!-- http://www.semanticweb.org/nazanin/ontologies/2025/Fairtology_L1#hasLiteraryMode -->

    <owl:ObjectProperty rdf:about="http://www.semanticweb.org/nazanin/ontologies/2025/Fairtology_L1#hasLiteraryMode">
        <rdfs:domain rdf:resource="http://example.org/fairytale#Fairytale"/>
        <rdfs:range rdf:resource="http://example.org/fairytale#LiteraryMode"/>
    </owl:ObjectProperty>
    


    <!-- http://www.semanticweb.org/nazanin/ontologies/2025/Fairtology_L1#hasMoralTheme -->

    <owl:ObjectProperty rdf:about="http://www.semanticweb.org/nazanin/ontologies/2025/Fairtology_L1#hasMoralTheme">
        <rdfs:domain rdf:resource="http://example.org/fairytale#Fairytale"/>
        <rdfs:range rdf:resource="http://example.org/fairytale#MoralTheme"/>
        <rdfs:comment>Links a tale to the moral lesson it conveys.</rdfs:comment>
    </owl:ObjectProperty>
    


    <!-- http://www.semanticweb.org/nazanin/ontologies/2025/Fairtology_L1#hasPlot -->

    <owl:ObjectProperty rdf:about="http://www.semanticweb.org/nazanin/ontologies/2025/Fairtology_L1#hasPlot">
        <rdfs:subPropertyOf rdf:resource="http://www.w3.org/2002/07/owl#topObjectProperty"/>
        <rdfs:domain rdf:resource="http://example.org/fairytale#Fairytale"/>
        <rdfs:range rdf:resource="http://example.org/fairytale#Plot"/>
    </owl:ObjectProperty>
    


    <!-- 
    ///////////////////////////////////////////////////////////////////////////////////////
    //
    // Data properties
    //
    ///////////////////////////////////////////////////////////////////////////////////////
     -->

    


    <!-- http://www.semanticweb.org/nazanin/ontologies/2025/Fairtology_L1#hasValue -->

    <owl:DatatypeProperty rdf:about="http://www.semanticweb.org/nazanin/ontologies/2025/Fairtology_L1#hasValue">
        <rdf:type rdf:resource="http://www.w3.org/2002/07/owl#FunctionalProperty"/>
        <rdfs:domain>
            <owl:Class>
                <owl:unionOf rdf:parseType="Collection">
                    <rdf:Description rdf:about="http://example.org/fairytale#MoralTheme"/>
                    <rdf:Description rdf:about="http://example.org/fairytale#Plot"/>
                </owl:unionOf>
            </owl:Class>
        </rdfs:domain>
        <rdfs:range rdf:resource="http://www.w3.org/2001/XMLSchema#string"/>
        <rdfs:comment>Plot of the Fairy tale or Moral theme contain strings</rdfs:comment>
        <rdfs:label xml:lang="en">hasValue</rdfs:label>
    </owl:DatatypeProperty>
    


    <!-- 
    ///////////////////////////////////////////////////////////////////////////////////////
    //
    // Classes
    //
    ///////////////////////////////////////////////////////////////////////////////////////
     -->

    


    <!-- http://example.org/fairytale#CharacterArchetype -->

    <owl:Class rdf:about="http://example.org/fairytale#CharacterArchetype">
        <rdfs:comment>Represents common character roles in fairy tales which were modeled based on a  simplified set of narrative character roles commonly found in fairy tales. This model draws conceptually from Northrop Frye&apos;s theory of literary archetypes but adapts it to the domain of folk and fairy tale ontology.</rdfs:comment>
    </owl:Class>
    


    <!-- http://example.org/fairytale#EndingType -->

    <owl:Class rdf:about="http://example.org/fairytale#EndingType">
        <rdfs:comment>Denotes the resolution structure or emotional closure of the story.</rdfs:comment>
    </owl:Class>
    


    <!-- http://example.org/fairytale#Fairytale -->

    <owl:Class rdf:about="http://example.org/fairytale#Fairytale">
        <rdfs:comment>Represents the original fairy tale narratives.</rdfs:comment>
    </owl:Class>
    


    <!-- http://example.org/fairytale#Helper -->

    <owl:Class rdf:about="http://example.org/fairytale#Helper">
        <rdfs:subClassOf rdf:resource="http://example.org/fairytale#CharacterArchetype"/>
        <rdfs:comment>Supports the hero through guidance or gifts.</rdfs:comment>
    </owl:Class>
    


    <!-- http://example.org/fairytale#Hero -->

    <owl:Class rdf:about="http://example.org/fairytale#Hero">
        <rdfs:subClassOf rdf:resource="http://example.org/fairytale#CharacterArchetype"/>
        <rdfs:comment>Central figure on a quest or journey.</rdfs:comment>
    </owl:Class>
    


    <!-- http://example.org/fairytale#IronicMode -->

    <owl:Class rdf:about="http://example.org/fairytale#IronicMode">
        <rdfs:subClassOf rdf:resource="http://example.org/fairytale#LiteraryMode"/>
        <rdfs:comment>A narrative where the characters are below the audience in knowledge or power; emphasizes irony, futility, or ambiguity.</rdfs:comment>
    </owl:Class>
    


    <!-- http://example.org/fairytale#LiteraryMode -->

    <owl:Class rdf:about="http://example.org/fairytale#LiteraryMode">
        <rdfs:comment>Narrative mode expressing the symbolic or emotional tone of a tale. Adapted from Fryeâ€™s typology of literary modes.</rdfs:comment>
    </owl:Class>
    


    <!-- http://example.org/fairytale#MoralTheme -->

    <owl:Class rdf:about="http://example.org/fairytale#MoralTheme">
        <rdfs:comment>Captures the ethical teachings conveyed through the narratives.</rdfs:comment>
    </owl:Class>
    


    <!-- http://example.org/fairytale#MythicMode -->

    <owl:Class rdf:about="http://example.org/fairytale#MythicMode">
        <rdfs:subClassOf rdf:resource="http://example.org/fairytale#LiteraryMode"/>
        <rdfs:comment>A narrative mode where characters are gods or superhuman beings; the setting is cosmic and timeless.</rdfs:comment>
    </owl:Class>
    


    <!-- http://example.org/fairytale#Plot -->

    <owl:Class rdf:about="http://example.org/fairytale#Plot">
        <rdfs:comment>Encapsulates the overall designed arrangement of story elements to produce an emotional or thematic effect.</rdfs:comment>
    </owl:Class>
    


    <!-- http://example.org/fairytale#RomanticMode -->

    <owl:Class rdf:about="http://example.org/fairytale#RomanticMode">
        <rdfs:subClassOf rdf:resource="http://example.org/fairytale#LiteraryMode"/>
        <rdfs:comment>A narrative mode in which the hero operates above ordinary limitations; idealized, heroic, or magical.</rdfs:comment>
    </owl:Class>
    


    <!-- http://example.org/fairytale#TragicMode -->

    <owl:Class rdf:about="http://example.org/fairytale#TragicMode">
        <rdfs:subClassOf rdf:resource="http://example.org/fairytale#LiteraryMode"/>
        <rdfs:comment>A narrative where the protagonist falls from a high position due to fate or personal flaw; evokes pity and fear.</rdfs:comment>
    </owl:Class>
    


    <!-- http://example.org/fairytale#Villain -->

    <owl:Class rdf:about="http://example.org/fairytale#Villain">
        <rdfs:subClassOf rdf:resource="http://example.org/fairytale#CharacterArchetype"/>
        <rdfs:comment>Antagonist who creates conflict or danger.</rdfs:comment>
    </owl:Class>
    


    <!-- http://www.semanticweb.org/nazanin/ontologies/2025/Fairtology_L1#Audience -->

    <owl:Class rdf:about="http://www.semanticweb.org/nazanin/ontologies/2025/Fairtology_L1#Audience">
        <rdfs:comment>Refers to the intended or actual viewers/readers of the tale.</rdfs:comment>
    </owl:Class>
    


    <!-- http://www.semanticweb.org/nazanin/ontologies/2025/Fairtology_L1#Bittersweet -->

    <owl:Class rdf:about="http://www.semanticweb.org/nazanin/ontologies/2025/Fairtology_L1#Bittersweet">
        <rdfs:subClassOf rdf:resource="http://example.org/fairytale#EndingType"/>
        <rdfs:comment>Mixed resolution involving growth through loss or sacrifice.</rdfs:comment>
    </owl:Class>
    


    <!-- http://www.semanticweb.org/nazanin/ontologies/2025/Fairtology_L1#HappilyEverAfter -->

    <owl:Class rdf:about="http://www.semanticweb.org/nazanin/ontologies/2025/Fairtology_L1#HappilyEverAfter">
        <rdfs:subClassOf rdf:resource="http://example.org/fairytale#EndingType"/>
        <rdfs:comment>Positive resolution, often involving marriage or restoration.</rdfs:comment>
    </owl:Class>
    


    <!-- http://www.semanticweb.org/nazanin/ontologies/2025/Fairtology_L1#Tragic -->

    <owl:Class rdf:about="http://www.semanticweb.org/nazanin/ontologies/2025/Fairtology_L1#Tragic">
        <rdfs:subClassOf rdf:resource="http://example.org/fairytale#EndingType"/>
        <rdfs:comment>Negative outcome involving loss or death.</rdfs:comment>
    </owl:Class>
    


    <!-- http://www.semanticweb.org/nazanin/ontologies/2025/Fairtology_L1#Trickster -->

    <owl:Class rdf:about="http://www.semanticweb.org/nazanin/ontologies/2025/Fairtology_L1#Trickster">
        <rdfs:subClassOf rdf:resource="http://example.org/fairytale#CharacterArchetype"/>
        <rdfs:comment>Character who disrupts or subverts norms through cleverness.</rdfs:comment>
    </owl:Class>
</rdf:RDF>



<!-- Generated by the OWL API (version 4.5.26.2023-07-17T20:34:13Z) https://github.com/owlcs/owlapi -->

